iris/SpecUservec.v
@@ -541,7 +541,7 @@ Definition wp_uservec_pt_body `{!riscvGS Σ, !xv6G Σ, !bioslotG Σ, !fileG Σ} 
     (ProcDefs.upd_usM (ProcInv.us_tf U (tf_of g (ret_pc sepc_v))) M) -∗
   (* ...and THE KILL ROW, owed at every cause and read only at the ones
      usertrap kills at ([SpecUsertrap.ut_kill_in]) *)
-  ut_kill_in f sc_v Wk gn -∗
+  ut_kill_in f sc_v Wk gn sts -∗
   wp_next true (proc_addr j) (fun CID' : CpuId =>
     uservec_post (CID := CID') (URes CID') C pt vksp U M g sts gn cs pid
       sepc_v sc_v f Wk) -∗
